# Quadratic equations

$$x = {-b \pm \sqrt{b^2-4ac} \over 2a}$$

$(a+b)^2$

$$\eqalign{
(a+b)^2 &= (a+b)(a+b) \\
        &= a^2 + ab + ba + b^2 \\
        &= a^2 + 2ab + b^2
}$$

$(a-b)^2$

$$\eqalign{
(a-b)^2 &= (a-b)(a-b) \\
        &= a^2 - ab - ba + b^2 \\
        &= a^2 - 2ab + b^2
}$$

$(a-b)(a+b)$

$$\eqalign{
(a+b)(a-b)  &= a^2 - ab + ba - b^2 \\
        &= a^2 - b^2
}$$

# Functions

$$ f(x) = {\sqrt{3x-1}+(1+x)^2 } $$


$$ g(x) = {\\frac{a}{1-a^2} }$$

$$ f(x) = {(x + 2) \over (2x + 1)} $$   


$$ f(x) = { \sqrt[3]{x^2} }$$
  
$$ \sqrt[5]{34}$$
  
# Trigonometry

$$ cos^2 \theta + sin^2 \theta  = 1  $$

Prove $ \sqrt{ 1 - cos^2 \theta \over 1- sin^2 \theta} = tan \theta $

$$ \sqrt{ 1 - cos^2 \theta \over 1- sin^2 \theta} = \sqrt{ sin^2 \theta \over cos^2 \theta} = {sin \theta \over cos \theta}  = Tan \theta $$

# Calculus

$$\eqalign{
f(x) = {3x^4} \implies {dy \over dx} = 12x^3
}$$

$$\eqalign{
f(x) = {2x^{-3/2}} \implies  {dy \over dx} = -3x^{-5/2} &= - {3 \over \sqrt{x^5}}
}$$

If $x = 2t + 1$ and $ y = t^2$ find ${dy \over dx}$ ?

$$\eqalign{
x = 2t + 1 \implies  {dx \over dt} = 2 \\
        y = t^2 \implies  {dy \over dt} = 2t \\
        {dy \over dx} = {dy \over dt} \div {dx \over dt} \\
         \implies 2t \div 2 = t
}$$

# Integration

Evaluate $\int_1^2 (x + 4)^2 dx $

$$\eqalign{
\int_1^2 (x + 4)^2 dx =  \int_1^2 (x^2 + 8x + 16) dx \\
        &= \left\lbrack {x^3 \over 3} + {8x^2 \over 2}  + 16x \right\rbrack_1^2 \\
        &= \left\lbrack {8 \over 3} + {8 * 4 \over 2}  + 16 * 2 \right\rbrack - \left\lbrack {1 \over 3} + {8 \over 2}  + 16  \right\rbrack 
}$$


# Links

https://github.blog/changelog/2022-05-19-render-mathematical-expressions-in-markdown/

https://www.mathjax.org/

http://docs.mathjax.org/en/latest/

https://docs.mathjax.org/en/v2.7-latest/tex.html

https://www.onemathematicalcat.org/MathJaxDocumentation/TeXSyntax.htm
